commit

AP/AP/Defense/Defs.lean
@@ -49,9 +49,26 @@ def merge (dse₁ dse₂ : Defense) : Defense where
 def ofList (ds : List Defense) : Defense :=
   ds.foldr merge ∅
 
-def Compatible (dse₁ dse₂ : Defense) : Prop :=
-  ∀ {s₀} [sys.WF s₀] {s p₁ p₂}, dse₁.cnd s₀ → dse₂.cnd s₀ → sys.Reachable s₀ s →
+def Compatible' (p : State → Prop) (dse₁ dse₂ : Defense) : Prop :=
+  ∀ {s₀} [sys.WF s₀] {s p₁ p₂}, p s₀ → dse₁.cnd s₀ → dse₂.cnd s₀ → sys.Reachable s₀ s →
   dse₁.f s = some p₁ → dse₂.f s = some p₂ → p₁ = p₂
 
+def Compatible (dse₁ dse₂ : Defense) : Prop :=
+  Compatible' (λ _ => True) dse₁ dse₂
+
+def CompatibleList' (p : State → Prop) (ds : List Defense) : Prop :=
+  ∀ {s₀} [sys.WF s₀] {s p₁ p₂ d₁ d₂}, p s₀ → (∀ d ∈ ds, d.cnd s₀) → sys.Reachable s₀ s →
+  d₁ ∈ ds → d₂ ∈ ds → d₁.f s = some p₁ → d₂.f s = some p₂ → p₁ = p₂
+
 def CompatibleList (ds : List Defense) : Prop :=
-  ∀ {e₁ e₂}, e₁ ∈ ds → e₂ ∈ ds → e₁.Compatible e₂
+  CompatibleList' (λ _ => True) ds
+
+def WF' (p : State → Prop) (dse : Defense) : Prop :=
+  ∀ {s} [sys.WF s], p s → dse.cnd s → ∀ (a : AStrat) [a.WF],
+  ∀ (d : DStrat) [d.WF] n, (sys.simulate (Strat.f ⟨a, dse.st d⟩) s n).1.aPos ∉ dse.ps
+
+-- def setCnd (d : Defense) (cnd : State → Prop) : Defense :=
+--   {d with cnd := cnd}
+-- 
+-- def accCndList (d : Defense) (ds : List Defense) : List Defense :=
+--   d.setCnd (∀ d₁, d₁ = d ∨ d₁ ∈ ds → d₁.cnd ·) :: ds.map (·.setCnd λ _ => True)
