AP/AP/Defense/Basic.lean
@@ -24,7 +24,7 @@ theorem valid_tr [H : dse.WF] {s} [DState s] {p} :
 dse.f s = some p → sys.validTr s p := H.1
 
 @[simp]
-instance [H : dse.WF] {d : DStrat} [Hd : d.WF] : (dse.st d).WF := by
+instance {d : DStrat} [H : dse.WF] [Hd : d.WF] : (dse.st d).WF := by
   unfold st; rw [DStrat.wf_iff]; intro s hs
   dsimp; cases h : dse.f s <;> simp; exact dse.valid_tr h
 
@@ -208,6 +208,9 @@ theorem merge_empty_right : merge dse ∅ = dse := by
 theorem st_merge : (dse₁.merge dse₂).st = λ d => dse₁.st (dse₂.st d) := by
   simp [merge]; delta st; simp
 
+theorem st_merge_ext {d} : (dse₁.merge dse₂).st d = dse₁.st (dse₂.st d) := by
+  simp
+
 @[simp]
 theorem validTr_merge_of_wf [H₁ : dse₁.WF] [H₂ : dse₂.WF] : (dse₁.merge dse₂).ValidTr := by
   intro s hs p hp
@@ -216,49 +219,28 @@ theorem validTr_merge_of_wf [H₁ : dse₁.WF] [H₂ : dse₂.WF] : (dse₁.merg
   · exact valid_tr hp
   · exact valid_tr h₂
 
-theorem wf_merge {e₁ e₂ : Defense} [He₁ : e₁.WF] [He₂ : e₂.WF]
-(h₀ : Compatible e₁ e₂) : (e₁.merge e₂).WF := by
-  use validTr_merge_of_wf
-  intro s hs h a Ha d Hd n
-  simp at h
-  rcases h with ⟨h₁, h₂⟩
-  have H₁ := He₁.2 h₁ a (e₂.st d) n
-  have H₂ := He₂.2 h₂ a (e₁.st d) n
-  generalize hr : sys.simulate (Strat.f ⟨a, e₁.st # e₂.st d⟩) s n = r at H₁
-  have h₃ : sys.simulate (Strat.f ⟨a, e₂.st # e₁.st d⟩) s n = r
-  · rw [←hr, ←Defense.simulate_st_comm]
-    intro s' h₃ p₁ p₂ h₄
-    have hs' := sys.wf_of_reachable h₃
-    intro h₅; exact @h₀ s _ s' p₁ p₂ h₁ h₂ h₃ h₄ h₅
-  rw [h₃] at H₂; clear h₃
-  have h₄ : sys.simulate (Strat.f ⟨a, (e₁.merge e₂).st d⟩) s n = r
-  · convert hr using 2; ext1 s
-    unfold Strat.f; split_ifs with ht <;> simp
-  rw [h₄]; simp [H₁, H₂]
-
 @[refl, simp]
 theorem Compatible.refl : dse.Compatible dse := by
-  simp [Compatible]; intros; simp_all only [Option.some.injEq]
+  simp [Compatible, Compatible']; intros; simp_all only [Option.some.injEq]
 
 @[symm]
 theorem Compatible.symm (h : dse₁.Compatible dse₂) : dse₂.Compatible dse₁ := by
-  simp [Compatible] at h ⊢
+  simp [Compatible, Compatible'] at h ⊢
   intro s₀ s p₁ p₂ hs h₁ h₂ h₃ h₄ h₅
   exact h h₂ h₁ h₃ h₅ h₄ |>.symm
 
 @[simp]
 theorem compatible_empty_left : Compatible ∅ dse := by
-  simp [Compatible]
+  simp [Compatible, Compatible']
 
 @[simp]
 theorem compatible_empty_right : Compatible dse ∅ := by
-  simp [Compatible]
+  simp [Compatible, Compatible']
 
 theorem compatible_merge_left_of {a b c} (h₁ : Compatible a c)
 (h₂ : Compatible b c) : Compatible (merge a b) c := by
-  intro s₀ s p₁ p₂ hs h₃ h₄ h₅ h₆ h₇
-  simp at h₃ h₆
-  rcases h₃ with ⟨ha, hb⟩
+  simp [Compatible, Compatible'] at h₁ h₂ ⊢
+  intro s₀ s p₁ p₂ h₀ ha hb h₄ h₅ h₆ h₇
   rcases h₆ with h₆ | ⟨h₆, h₈⟩
   · exact h₁ ha h₄ h₅ h₆ h₇
   · exact h₂ hb h₄ h₅ h₈ h₇
@@ -267,7 +249,7 @@ theorem compatible_merge_right_of {a b c} (h₁ : Compatible a b)
 (h₂ : Compatible a c) : Compatible a (merge b c) := by
   symm at *; exact compatible_merge_left_of h₁ h₂
 
-theorem compatible_ofList_of {e : Defense} {ds : List Defense}
+theorem compatible_ofList_of_forall_compatible {e : Defense} {ds : List Defense}
 (h : ∀ e₁ ∈ ds, e.Compatible e₁) : e.Compatible (ofList ds) := by
   induction ds; simp
   nm e' ds ih
@@ -276,41 +258,44 @@ theorem compatible_ofList_of {e : Defense} {ds : List Defense}
   specialize @ih h₂
   simp; exact compatible_merge_right_of h₁ ih
 
+-- theorem compatibleList_of_compatibleList_cons {d ds}
+-- (h : CompatibleList (d :: ds)) : CompatibleList ds := by
+--   intros s₀ hs₀ s p₁ p₂ d₁ d₂ h₁ h₂ h₃ h₄ h₅ h₆
+--   specialize @h s₀ _ s p₁ p₂ d₁ d₂
+--   simp at h
+
+-- #check 0 #exit
+
+-- theorem compatible_ofList_of_compatibleList {d : Defense} {ds : List Defense}
+-- (h : CompatibleList (d :: ds)) : d.Compatible (ofList ds) := by
+--   induction ds; simp
+--   nm d' ds ih
+--   simp
+
+-- #check 0 #exit
+
 @[simp]
 theorem compatibleList_nil : CompatibleList [] := by
-  simp [CompatibleList]
+  simp [CompatibleList, CompatibleList']
 
-@[simp]
-theorem compatibleList_cons {e ds} :
-CompatibleList (e :: ds) ↔ CompatibleList ds ∧ ∀ e₁ ∈ ds, e.Compatible e₁ := by
-  simp [CompatibleList]
-  constructor
-  · intro h
-    split_ands
-    · intro e₁ e₂ he₁ he₂
-      specialize @h e₁ e₂
-      simp [he₁, he₂] at h
-      exact h
-    · intro e₁ he₁
-      specialize @h e e₁
-      simp [he₁] at h
-      exact h
-  · rintro ⟨h₁, h₂⟩ e₁ e₂ (rfl | he₁) (rfl | he₂)
-    · rfl
-    · exact h₂ _ he₂
-    · symm; exact h₂ _ he₁
-    · exact h₁ he₁ he₂
-
-theorem wf_ofList {ds : List Defense} (H : ∀ d ∈ ds, d.WF)
-(h₀ : CompatibleList ds) : (ofList ds).WF := by
-  induction ds <;> simp
-  nm e ds ih
-  simp only [List.mem_cons, forall_eq_or_imp, compatibleList_cons] at H h₀
-  rcases H with ⟨He, H⟩
-  rcases h₀ with ⟨h₁, h₂⟩
-  specialize ih H h₁
-  apply wf_merge
-  exact compatible_ofList_of h₂
+-- theorem compatible_of_compatibleList {ds d₁ d₂} (h : CompatibleList ds)
+-- (h₁ : d₁ ∈ ds) (h₂ : d₂ ∈ ds) : Compatible d₁ d₂ := by
+--   unfold CompatibleList at h
+-- 
+-- #check 0 #exit
+-- 
+-- theorem of_compatibleList_cons {e ds} (h : CompatibleList (e :: ds)) :
+-- CompatibleList ds ∧ ∀ e₁ ∈ ds, e.Compatible e₁ := by
+--   simp [CompatibleList]
+--   split_ands
+--   · intro e₁ e₂ he₁ he₂
+--     specialize @h e₁ e₂
+--     simp [he₁, he₂] at h
+--     exact h
+--   · intro e₁ he₁
+--     specialize @h e e₁
+--     simp [he₁] at h
+--     exact h
 
 @[simp]
 theorem validTr_empty : ValidTr ∅ := by
@@ -336,21 +321,236 @@ theorem validTr_ofList {ds : List Defense}
 (H : ∀ d ∈ ds, d.WF) : (ofList ds).ValidTr :=
   validTr_ofList' # λ d hd => H d hd |>.1
 
-theorem compatibleList_iff_getElem {ds : List Defense} :
-CompatibleList ds ↔ ∀ i j (h₁ : i < j) (h₂ : j < ds.length), ds[i].Compatible ds[j] := by
-  unfold CompatibleList
-  constructor
-  · intro h i j h₁ h₂
-    apply @h ds[i] ds[j] <;> simp
-  intro h e₁ e₂ h₁ h₂
-  rw [List.mem_iff_getElem] at h₁ h₂
-  obtain ⟨i, h₁, rfl⟩ := h₁
-  obtain ⟨j, h₂, rfl⟩ := h₂
-  rcases lt_trichotomy i j with h₃ | rfl | h₃
-  on_goal 2 => rfl
-  · apply h; exact h₃
-  · symm; apply h; exact h₃
+@[simp]
+theorem merge_self {d} : merge d d = d := by
+  simp [merge]
 
-theorem compatibleList_iff_getElem! {ds : List Defense} :
-CompatibleList ds ↔ ∀ i j, i < j → j < ds.length → ds[i]!.Compatible ds[j]! := by
-  convert compatibleList_iff_getElem <;> apply getElem!_pos
+theorem merge_assoc {a b c} : merge (merge a b) c = merge a (merge b c) := by
+  simp [merge, and_assoc, Set.union_assoc, Option.or_assoc]
+
+@[simp]
+theorem ofList_append {ds₁ ds₂} : ofList (ds₁ ++ ds₂) = merge (ofList ds₁) (ofList ds₂) := by
+  induction ds₁ <;> simp; nm d ds₁ ih; simp [ih, merge_assoc]
+
+@[simp]
+theorem cnd_ofList {ds s} : (ofList ds).cnd s ↔ ∀ d ∈ ds, d.cnd s := by
+  induction ds <;> simp; grind
+
+@[simp]
+theorem ps_ofList {ds} : (ofList ds).ps = ⋃ d ∈ ds, d.ps := by
+  induction ds <;> simp; grind
+
+@[simp]
+theorem st_empty : (∅ : Defense).st = id := by
+  ext:1; simp [st]
+
+theorem compatibleList'_of_perm {p} {ds₁ ds₂ : List Defense}
+(h₁ : CompatibleList' p ds₁) (h₂ : ds₁.Perm ds₂) : CompatibleList' p ds₂ := by
+  unfold CompatibleList' at h₁ ⊢; grind
+
+theorem compatibleList_of_perm {ds₁ ds₂ : List Defense}
+(h₁ : CompatibleList ds₁) (h₂ : ds₁.Perm ds₂) : CompatibleList ds₂ :=
+  compatibleList'_of_perm h₁ h₂
+
+theorem compatibleList'_iff_of_perm {p} {ds₁ ds₂ : List Defense}
+(h : ds₁.Perm ds₂) : CompatibleList' p ds₁ ↔ CompatibleList' p ds₂ :=
+  ⟨λ h₁ => compatibleList'_of_perm h₁ h, λ h₁ => compatibleList'_of_perm h₁ h.symm⟩
+
+theorem compatibleList_iff_of_perm {ds₁ ds₂ : List Defense}
+(h : ds₁.Perm ds₂) : CompatibleList ds₁ ↔ CompatibleList ds₂ :=
+  compatibleList'_iff_of_perm h
+
+theorem of_compatibleList'_cons {p d ds} (h : CompatibleList' p (d :: ds)) :
+CompatibleList' (λ s => d.cnd s ∧ p s) ds := by
+  unfold CompatibleList' at h ⊢; grind
+
+theorem of_compatibleList_cons {d ds} (h : CompatibleList (d :: ds)) :
+CompatibleList' d.cnd ds := by
+  have h₁ := @of_compatibleList'_cons (h := h)
+  simp at h₁; simp_all only
+
+theorem of_f_of_list_eq_some {ds s p} (h : (ofList ds).f s = some p) :
+∃ d ∈ ds, d.f s = some p := by
+  induction ds <;> simp_all; grind
+
+theorem wf_merge {e₁ e₂ : Defense} [He₁ : e₁.WF] [He₂ : e₂.WF]
+(h₀ : Compatible e₁ e₂) : (e₁.merge e₂).WF := by
+  use validTr_merge_of_wf
+  intro s hs h a Ha d Hd n
+  simp at h
+  rcases h with ⟨h₁, h₂⟩
+  have H₁ := He₁.2 h₁ a (e₂.st d) n
+  have H₂ := He₂.2 h₂ a (e₁.st d) n
+  generalize hr : sys.simulate (Strat.f ⟨a, e₁.st # e₂.st d⟩) s n = r at H₁
+  have h₃ : sys.simulate (Strat.f ⟨a, e₂.st # e₁.st d⟩) s n = r
+  · rw [←hr, ←simulate_st_comm]
+    intro s' h₃ p₁ p₂ h₄
+    have hs' := sys.wf_of_reachable h₃
+    intro h₅; exact @h₀ s _ s' p₁ p₂ (by simp) h₁ h₂ h₃ h₄ h₅
+  rw [h₃] at H₂; clear h₃
+  have h₄ : sys.simulate (Strat.f ⟨a, (e₁.merge e₂).st d⟩) s n = r
+  · convert hr using 2; ext1 s
+    unfold Strat.f; split_ifs with ht <;> simp
+  rw [h₄]; simp [H₁, H₂]
+
+theorem wf_iff_validTr_and_wf' {d : Defense} : d.WF ↔ d.ValidTr ∧ d.WF' (λ _ => True) := by
+  simp [WF']; constructor
+  · intro h; cases h; nm h₁ h₂; use h₁
+  · rintro ⟨h₁, h₂⟩; use h₁
+
+-- @[simp] theorem cnd_setCnd {d cnd} : (setCnd d cnd).cnd = cnd := rfl
+-- @[simp] theorem ps_setCnd {d cnd} : (setCnd d cnd).ps = d.ps := rfl
+-- @[simp] theorem f_setCnd {d cnd} : (setCnd d cnd).f = d.f := rfl
+-- 
+-- @[simp]
+-- theorem ofList_accCndList {d ds} : ofList (accCndList d ds) = ofList (d :: ds) := by
+--   unfold accCndList; ext:1 <;> simp; ext s p :2; simp; induction ds <;> simp; grind
+-- 
+-- @[simp]
+-- theorem length_accCndList {d ds} : (accCndList d ds).length = ds.length + 1 := by
+--   simp [accCndList]
+
+theorem wf_dStrat_of_validTr {d : DStrat} [Hd : d.WF] (h : dse.ValidTr) : (dse.st d).WF := by
+  unfold st; rw [DStrat.wf_iff]; intro s hs
+  dsimp; cases h₁ : dse.f s <;> simp; exact h h₁
+
+@[simp]
+theorem compatibleList'_nil {p} : CompatibleList' p [] := by
+  simp [CompatibleList']
+
+theorem compatibleList'_append_comm {p ds₁ ds₂} :
+CompatibleList' p (ds₁ ++ ds₂) ↔ CompatibleList' p (ds₂ ++ ds₁) :=
+  compatibleList'_iff_of_perm List.perm_append_comm
+
+theorem right_of_compatibleList'_append {p ds₁ ds₂} (h : CompatibleList' p (ds₁ ++ ds₂)) :
+CompatibleList' (λ s => (∀ d ∈ ds₁, d.cnd s) ∧ p s) ds₂ := by
+  induction ds₁ generalizing ds₂ p
+  · simp at h ⊢; simp_all only
+  nm d ds₁ ih
+  simp
+  replace h := @of_compatibleList'_cons (h := h)
+  specialize @ih _ _ h
+  clear h
+  grind
+
+theorem left_of_compatibleList'_append {p ds₁ ds₂} (h : CompatibleList' p (ds₁ ++ ds₂)) :
+CompatibleList' (λ s => (∀ d ∈ ds₂, d.cnd s) ∧ p s) ds₁ := by
+  rw [compatibleList'_append_comm] at h
+  exact right_of_compatibleList'_append h
+
+theorem wf'_of_imp {d p₁ p₂} (h₁ : WF' p₁ d) (h₂ : ∀ s, p₂ s → p₁ s) : WF' p₂ d := by
+  unfold WF' at h₁ ⊢; grind
+
+theorem simulate_st_comm' {s₀ n} {a : AStrat} {d : DStrat}
+[hs₀ : sys.WF s₀] [Ha : a.WF] [Hd : d.WF]
+(hv₁ : dse₁.ValidTr) (hv₂ : dse₂.ValidTr)
+(h : ∀ s, sys.Reachable s₀ s → ∀ {p₁ p₂},
+dse₁.f s = some p₁ → dse₂.f s = some p₂ → p₁ = p₂) :
+sys.simulate (Strat.f ⟨a, dse₁.st (dse₂.st d)⟩) s₀ n =
+sys.simulate (Strat.f ⟨a, dse₂.st (dse₁.st d)⟩) s₀ n := by
+  have G₁ : dse₁.st d |>.WF; exact wf_dStrat_of_validTr hv₁
+  have G₀ : dse₂.st d |>.WF; exact wf_dStrat_of_validTr hv₂
+  have G₂ : dse₁.st (dse₂.st d) |>.WF; exact wf_dStrat_of_validTr hv₁
+  have G₃ : dse₂.st (dse₁.st d) |>.WF; exact wf_dStrat_of_validTr hv₂
+  apply simulate_congr <;> simp
+  intro k hk s hs h₁ h₂ h₃
+  simp [st]
+  cases H₃ : dse₁.f s <;> cases H₄ : dse₂.f s <;> simp
+  nm p₁ p₂
+  have H₅ := sys.reachable_of_simulate_eq h₁
+  exact @h s H₅ p₁ p₂ H₃ H₄
+
+theorem wf_ofList {ds : List Defense} (H : ∀ d ∈ ds, d.WF)
+(h₀ : CompatibleList ds) : (ofList ds).WF := by
+  rw [wf_iff_validTr_and_wf']
+  generalize hp : (λ s => True) = p at h₀
+  replace H : ∀ d ∈ ds, d.ValidTr ∧ d.WF' p
+  · simp [←hp]
+    simp_rw [wf_iff_validTr_and_wf'] at H
+    exact H
+  unfold CompatibleList at h₀
+  rw [hp] at h₀
+  clear hp
+  generalize hN : ds.length = N
+  induction N using Nat.strong_induction_on generalizing ds p
+  nm N IH
+  use validTr_ofList' # by grind
+  intro s₀ hs₀ G h a Ha d Hd n
+  generalize hr : sys.simulate (Strat.f ⟨a, (ofList ds).st d⟩) s₀ n = r
+  rcases r with ⟨s, r⟩
+  have hx := sys.reachable_of_simulate_eq hr
+  simp
+  intro e he
+  replace he := List.eq_append_cons_of_mem he
+  obtain ⟨ds₁, ds₂, hds, -⟩ := he
+  generalize hds' : e :: (ds₁ ++ ds₂) = ds'
+  have H₁ : ds.Perm ds'
+  · simp [hds, ←hds']
+  simp [hds] at hr
+  generalize hd' : (ofList ds₂).st d = d' at hr
+  replace hd' : d'.WF
+  · simp [←hd']
+    apply wf_dStrat_of_validTr
+    apply validTr_ofList'
+    simp [hds] at H
+    grind
+  clear Hd d
+  rename' d' => d, hd' => hd
+  generalize H₂ : ofList ds₁ = e₁ at hr
+  obtain ⟨he', he⟩ : e.ValidTr ∧ e.WF' p
+  · grind
+  rw [hds] at h₀
+  have h₀' := @left_of_compatibleList'_append (h := h₀)
+  generalize hp' : (λ s => (∀ d ∈ e :: ds₂, d.cnd s) ∧ p s) = p'
+  obtain ⟨he₁', he₁⟩ : e₁.ValidTr ∧ e₁.WF' p'
+  · subst H₂ hp'
+    apply @IH ds₁.length (by grind) ds₁ _ h₀' _ rfl
+    intro y hy
+    simp [hds] at H
+    specialize H y
+    simp [hy] at H
+    rcases H with ⟨H₃, H₄⟩
+    use H₃
+    apply wf'_of_imp H₄
+    simp
+  have hd₁ : e₁.st d |>.WF
+  · exact wf_dStrat_of_validTr he₁'
+  rw [simulate_st_comm'] at hr
+  rotate_left
+  · grind
+  · grind
+  · intro s₁ hs₁ p₁ p₂ hp₁ hp₂
+    simp [←H₂] at hp₁
+    replace hp₁ := of_f_of_list_eq_some hp₁
+    choose e₂ H₃ hp₁ using hp₁
+    specialize @h₀ s₀ _ s₁ p₁ p₂ e₂ e _ _ hs₁
+    · simp [hds] at h; grind
+    · simp [hds] at h; grind
+    simp [H₃, hp₁, hp₂] at h₀
+    exact h₀
+  specialize @he s₀ _ G _ a _ (e₁.st d) _ n
+  · simp [hds] at h
+    grind
+  simp [hr] at he
+  exact he
+
+-- #check 0 #exit
+
+-- theorem compatibleList_iff_getElem {ds : List Defense} :
+-- CompatibleList ds ↔ ∀ i j (h₁ : i < j) (h₂ : j < ds.length), ds[i].Compatible ds[j] := by
+--   unfold CompatibleList
+--   constructor
+--   · intro h i j h₁ h₂
+--     apply @h ds[i] ds[j] <;> simp
+--   intro h e₁ e₂ h₁ h₂
+--   rw [List.mem_iff_getElem] at h₁ h₂
+--   obtain ⟨i, h₁, rfl⟩ := h₁
+--   obtain ⟨j, h₂, rfl⟩ := h₂
+--   rcases lt_trichotomy i j with h₃ | rfl | h₃
+--   on_goal 2 => rfl
+--   · apply h; exact h₃
+--   · symm; apply h; exact h₃
+
+-- theorem compatibleList_iff_getElem! {ds : List Defense} :
+-- CompatibleList ds ↔ ∀ i j, i < j → j < ds.length → ds[i]!.Compatible ds[j]! := by
+--   convert compatibleList_iff_getElem <;> apply getElem!_pos
